Ordinal/CantorNotation.v
@@ -1,0 +1,1312 @@
+Require Import Morphisms.
+Require Import Coq.Program.Basics.
+Require Import NArith.
+Require Import List.
+
+Unset Printing Records.
+
+From Ordinal Require Import Defs.
+From Ordinal Require Import Operators.
+From Ordinal Require Import Arith.
+From Ordinal Require Import Cantor.
+From Ordinal Require Import Fixpoints.
+From Ordinal Require Import Reflection.
+
+Open Scope ord_scope.
+
+Inductive CantorForm : Set :=
+  | CantorSum : list CantorForm -> CantorForm.
+
+Fixpoint cantorOrd (cf:CantorForm) : Ord :=
+  match cf with
+  | CantorSum xs =>
+      fold_right (fun (x:CantorForm) o => expOrd ω (cantorOrd x) + o) 0 xs
+  end.
+
+Canonical Structure CF :=
+  ord CantorForm cantorOrd.
+
+Import ListNotations.
+Open Scope list.
+
+Inductive ordering := LT | EQ | GT.
+
+Definition ordering_swap (o:ordering) : ordering :=
+  match o with
+  | LT => GT
+  | EQ => EQ
+  | GT => LT
+  end.
+
+Definition lexCompare (o1:ordering) (o2:ordering) : ordering :=
+  match o1 with
+  | LT => LT
+  | EQ => o2
+  | GT => GT
+  end.
+
+Fixpoint cantorCompare (x:CantorForm) (y:CantorForm) {struct x} : ordering :=
+  match x, y with
+  | CantorSum xs0, CantorSum ys0 =>
+    (fix cantorSumCompare (xs:list CantorForm) (ys:list CantorForm) {struct xs} : ordering :=
+       match xs, ys with
+       | [], [] => EQ
+       | [], (y::ys) => LT
+       | (x::xs), [] => GT
+       | (x::xs), (y::ys) =>
+         lexCompare (cantorCompare x y) (cantorSumCompare xs ys)
+       end) xs0 ys0
+  end.
+
+Definition cantorSumCompare : list CantorForm -> list CantorForm -> ordering :=
+  fix cantorSumCompare (xs:list CantorForm) (ys:list CantorForm) {struct xs} : ordering :=
+  match xs, ys with
+  | [], [] => EQ
+  | [], (y::ys) => LT
+  | (x::xs), [] => GT
+  | (x::xs), (y::ys) =>
+    lexCompare (cantorCompare x y) (cantorSumCompare xs ys)
+  end.
+
+Lemma cantorCompare_unfold xs ys : cantorCompare (CantorSum xs) (CantorSum ys) = cantorSumCompare xs ys.
+Proof.
+  reflexivity.
+Qed.
+
+
+Fixpoint cantorIsNormal (cf:CantorForm) : Prop :=
+  match cf with
+  | CantorSum [] => True
+  | CantorSum (x0::xs0) => cantorIsNormal x0 /\
+    (fix check (x:CantorForm) (xs:list CantorForm) : Prop :=
+      match xs with
+      | [] => True
+      | (x'::xs') => cantorIsNormal x' /\ cantorCompare x x' <> LT /\ check x' xs'
+      end) x0 xs0
+  end.
+
+Definition CantorNormalForm : Set := { cf:CantorForm | cantorIsNormal cf }.
+
+Definition CNF_denote (x:CantorNormalForm) := cantorOrd (proj1_sig x).
+
+Canonical Structure CNF := ord CantorNormalForm CNF_denote.
+
+Lemma cantorCompare_swap : forall (x y:CantorForm),
+  cantorCompare x y = ordering_swap (cantorCompare y x).
+Proof.
+  fix Hind 1.
+  intros [xs] [ys].
+  revert ys.
+  induction xs as [|x xs]; intros.
+  - destruct ys as [|y ys]; simpl in *; auto.
+  - destruct ys as [|y ys]; simpl in *; auto.
+    replace (cantorCompare x y) with (ordering_swap (cantorCompare y x)).
+    + destruct (cantorCompare y x); simpl in * ; auto.
+    + symmetry. apply Hind.
+Qed.
+
+Lemma CantorForm_complete : forall a, complete (cantorOrd a).
+Proof.
+  fix Hind 1.
+  intros [ls]. simpl.
+  induction ls.
+  - apply zero_complete.
+  - simpl fold_right.
+    apply addOrd_complete; auto.
+    apply expOrd_complete; auto.
+    apply (index_lt ω 0%nat).
+    apply omega_complete.
+Qed.
+
+Lemma cantorOrd_shrink : forall x, cantorOrd x < expOrd ω (cantorOrd x).
+Proof.
+  fix Hind 1.
+  intros [xs]. revert xs.
+  fix Hind_xs 1.
+  intros [|x xs].
+  - simpl cantorOrd.
+    apply expOrd_nonzero.
+  - simpl cantorOrd.
+    apply expOmega_additively_closed.
+    + apply (CantorForm_complete (CantorSum (x::xs))).
+    + rewrite expOrd_add.
+      apply ord_lt_le_trans with (expOrd ω (expOrd ω (cantorOrd x)) * 1).
+      rewrite mulOrd_one_r.
+      apply expOrd_increasing. apply omega_gt1.
+      apply Hind.
+      apply mulOrd_monotone2.
+      apply succ_least. apply expOrd_nonzero.
+    + rewrite expOrd_add.
+      apply ord_lt_le_trans with
+          (1 * expOrd ω (fold_right
+                           (fun (x0 : CantorForm) (o : Ord) => expOrd ω (cantorOrd x0) + o) 0 xs)).
+      rewrite mulOrd_one_l.
+      apply (Hind_xs xs).
+      apply mulOrd_monotone1.
+      apply succ_least. apply expOrd_nonzero.
+Qed.
+
+Lemma epslion_additively_closed : forall x, complete x -> additively_closed (ε x).
+Proof.
+  intros. hnf; intros.
+  rewrite ε_fixpoint.
+  apply expOmega_additively_closed.
+  - apply ε_complete; auto.
+  - rewrite <- ε_fixpoint. auto.
+  - rewrite <- ε_fixpoint. auto.
+Qed.
+
+Theorem cantorForm_below_epsilon : forall (x:CF), x < ε 0.
+Proof.
+  induction x using size_induction.
+  destruct x as [xs].
+  unfold sz. simpl ordSize.
+  induction xs.
+  - simpl fold_right.
+    rewrite ε_fixpoint.
+    apply expOrd_nonzero.
+  - simpl fold_right.
+    apply epslion_additively_closed.
+    apply zero_complete.
+    rewrite ε_fixpoint.
+    apply expOrd_increasing.
+    apply omega_gt1.
+    apply H.
+    simpl.
+    rewrite <- addOrd_le1.
+    apply cantorOrd_shrink.
+    apply IHxs.
+    intros.
+    apply H.
+    simpl.
+    rewrite <- addOrd_le2.
+    auto.
+Qed.
+
+
+Definition CantorNormalForm_lt (x y:CantorNormalForm) :=
+  cantorCompare (proj1_sig x) (proj1_sig y) = LT.
+
+Definition CantorNormalForm_le (x y:CantorNormalForm) :=
+  cantorCompare (proj1_sig x) (proj1_sig y) <> GT.
+
+Lemma CNF_compare_correct_lemma1 : forall
+  (lsa : list CantorForm)
+  (a : CantorForm)
+  (c : CantorForm)
+  (H : cantorIsNormal (CantorSum (a :: lsa)))
+  (Hlsa : cantorIsNormal (CantorSum lsa))
+  (Hc : cantorIsNormal c)
+  (H1 : cantorOrd a < cantorOrd c)
+  (Hind : forall y : CF,
+          (y ◃ CantorSum lsa) ->
+          forall b : CF,
+          cantorIsNormal y ->
+          cantorIsNormal b ->
+          match cantorCompare y b with
+          | LT => cantorOrd y < cantorOrd b
+          | EQ => cantorOrd y ≈ cantorOrd b
+          | GT => cantorOrd b < cantorOrd y
+          end),
+  fold_right (fun (x : CantorForm) (o : Ord) => expOrd ω (cantorOrd x) + o) 0
+    lsa < expOrd ω (cantorOrd c).
+Proof.
+  induction lsa; simpl; intros.
+  * apply expOrd_nonzero.
+  * apply expOmega_additively_closed.
+    apply CantorForm_complete.
+    apply expOrd_increasing; auto.
+    apply omega_gt1.
+    intuition.
+    apply ord_le_lt_trans with (cantorOrd a0); auto.
+    assert (match cantorCompare a a0 with
+            | LT => cantorOrd a < cantorOrd a0
+            | EQ => cantorOrd a ≈ cantorOrd a0
+            | GT => cantorOrd a0 < cantorOrd a
+            end).
+    apply Hind; auto.
+    { rewrite <- addOrd_le1. apply cantorOrd_shrink. }
+    rewrite cantorCompare_swap in H2.
+    destruct (cantorCompare a a0); intuition.
+    apply H5.
+    apply IHlsa with a; auto.
+    { clear -Hlsa; simpl in *; destruct lsa; intuition. }
+
+    intuition.
+    apply ord_le_lt_trans with (cantorOrd a0); auto.
+    assert (match cantorCompare a a0 with
+            | LT => cantorOrd a < cantorOrd a0
+            | EQ => cantorOrd a ≈ cantorOrd a0
+            | GT => cantorOrd a0 < cantorOrd a
+            end).
+    apply Hind; auto.
+    { rewrite <- addOrd_le1. apply cantorOrd_shrink. }
+    rewrite cantorCompare_swap in H2.
+    destruct (cantorCompare a a0); intuition.
+    apply H5.
+
+    intros; apply Hind; auto.
+    rewrite <- addOrd_le2; auto.
+Qed.
+
+Lemma CNF_compare_correct_lemma2 : forall
+  (a : CantorForm)
+  (Hind : forall y : CF,
+         y ◃ a ->
+         forall b : CF,
+         cantorIsNormal y ->
+         cantorIsNormal b ->
+         match cantorCompare y b with
+         | LT => cantorOrd y < cantorOrd b
+         | EQ => cantorOrd y ≈ cantorOrd b
+         | GT => cantorOrd b < cantorOrd y
+         end)
+  (lsb : list CantorForm)
+  (c : CantorForm)
+  (H0 : cantorIsNormal (CantorSum (c :: lsb)))
+  (Ha : cantorIsNormal a)
+  (Hc : cantorIsNormal c)
+  (H1 : cantorOrd c < cantorOrd a),
+  fold_right (fun (x : CantorForm) (o : Ord) => expOrd ω (cantorOrd x) + o) 0
+    lsb < expOrd ω (cantorOrd a).
+Proof.
+  intros a Hind. induction lsb; simpl fold_right; intros.
+  - apply expOrd_nonzero.
+  - apply expOmega_additively_closed.
+    apply CantorForm_complete.
+    apply expOrd_increasing; auto.
+    apply omega_gt1.
+    intuition.
+    apply ord_le_lt_trans with (cantorOrd c); auto.
+    assert (match cantorCompare c a0 with
+            | LT => cantorOrd c < cantorOrd a0
+            | EQ => cantorOrd c ≈ cantorOrd a0
+            | GT => cantorOrd a0 < cantorOrd c
+            end).
+    apply Hind; auto.
+    { simpl in H0. intuition. }
+    simpl in H0.
+    intuition.
+    destruct (cantorCompare c a0); intuition; auto with ord.
+    apply H.
+
+    apply IHlsb with a0; simpl in *; intuition.
+    apply ord_le_lt_trans with (cantorOrd c); auto.
+    assert (match cantorCompare c a0 with
+            | LT => cantorOrd c < cantorOrd a0
+            | EQ => cantorOrd c ≈ cantorOrd a0
+            | GT => cantorOrd a0 < cantorOrd c
+            end).
+    apply Hind; auto.
+    destruct (cantorCompare c a0); intuition; auto with ord.
+    apply H3.
+Qed.
+
+Lemma CNF_compare_correct :
+  forall (a b:CF),
+    cantorIsNormal a ->
+    cantorIsNormal b ->
+    match cantorCompare a b with
+    | LT => cantorOrd a < cantorOrd b
+    | EQ => cantorOrd a ≈ cantorOrd b
+    | GT => cantorOrd a > cantorOrd b
+    end.
+Proof.
+  induction a as [[xs] Hind] using size_induction.
+  induction xs as [|a lsa].
+  - intros [lsb]; destruct lsb; simpl; intros; auto with ord.
+    + reflexivity.
+    + rewrite <- addOrd_le1.
+      apply expOrd_nonzero.
+  - intros [lsb]; destruct lsb; intros.
+    + simpl.
+      rewrite <- addOrd_le1.
+      apply expOrd_nonzero.
+    + simpl cantorCompare.
+      assert (Hlsa : cantorIsNormal (CantorSum lsa)).
+      { simpl in H. simpl. destruct lsa; intuition. }
+      assert (Hlsb : cantorIsNormal (CantorSum lsb)).
+      { simpl in H0. simpl. destruct lsb; intuition. }
+      assert (Ha : cantorIsNormal a).
+      { simpl in H; intuition. }
+      assert (Hc : cantorIsNormal c).
+      { simpl in H0; intuition. }
+      assert (Hlt : a ◃ (CantorSum (a :: lsa))).
+      { simpl. rewrite <- addOrd_le1. apply cantorOrd_shrink. }
+      generalize (Hind a Hlt c Ha Hc).
+      destruct (cantorCompare a c); simpl.
+      * intros.
+        eapply ord_lt_le_trans; [ | apply addOrd_le1 ].
+        apply expOmega_additively_closed.
+        apply CantorForm_complete.
+        apply expOrd_increasing; auto.
+        apply omega_gt1.
+
+        apply CNF_compare_correct_lemma1 with a; auto.
+        intros; apply Hind; auto.
+        simpl. rewrite <- addOrd_le2; auto.
+
+      * intro Hac.
+        assert (match cantorCompare (CantorSum lsa) (CantorSum lsb) with
+                  | LT => cantorOrd (CantorSum lsa) < cantorOrd (CantorSum lsb)
+                  | EQ => cantorOrd (CantorSum lsa) ≈ cantorOrd (CantorSum lsb)
+                  | GT => cantorOrd (CantorSum lsb) < cantorOrd (CantorSum lsa)
+                end).
+        apply IHlsa; auto.
+        { intros. apply Hind; auto. simpl.
+          rewrite <- addOrd_le2. auto. }
+        simpl in H1.
+        destruct ((fix cantorSumCompare (xs ys : list CantorForm) {struct xs} : ordering :=
+            match xs with
+            | [] => match ys with
+                    | [] => EQ
+                    | _ :: _ => LT
+                    end
+            | x :: xs0 =>
+                match ys with
+                | [] => GT
+                | y :: ys0 =>
+                    lexCompare (cantorCompare x y) (cantorSumCompare xs0 ys0)
+                end
+            end) lsa lsb).
+        ** apply ord_le_lt_trans with
+            (expOrd ω (cantorOrd c) +
+                      fold_right (fun (x : CantorForm) (o : Ord) => expOrd ω (cantorOrd x) + o) 0 lsa).
+           apply addOrd_monotone; auto with ord.
+           apply expOrd_monotone; apply Hac.
+           apply addOrd_increasing. auto.
+        ** intros.
+           apply addOrd_eq_mor; auto.
+           split; apply expOrd_monotone; apply Hac.
+        ** apply ord_le_lt_trans with
+               (expOrd ω (cantorOrd a) +
+                fold_right (fun (x : CantorForm) (o : Ord) => expOrd ω (cantorOrd x) + o) 0 lsb).
+           apply addOrd_monotone; auto with ord.
+           apply expOrd_monotone; apply Hac.
+           apply addOrd_increasing. auto.
+
+      * intros.
+        eapply ord_lt_le_trans; [ | apply addOrd_le1 ].
+        apply expOmega_additively_closed.
+        apply CantorForm_complete.
+        apply expOrd_increasing; auto.
+        apply omega_gt1.
+        apply CNF_compare_correct_lemma2 with c; auto.
+        intros; apply Hind; auto.
+        simpl. rewrite <- addOrd_le1.
+        transitivity (sz a); auto.
+        apply cantorOrd_shrink.
+Qed.
+
+Lemma CNF_lt_reflects : reflects CantorNormalForm CNF_denote (Arrow ORD (Arrow ORD PROP)) ord_lt CantorNormalForm_lt.
+Proof.
+  simpl. intros x [a Ha] Hxa y [b Hb] Hyb.
+  unfold CNF_denote, CantorNormalForm_lt in *; simpl in *.
+  generalize (CNF_compare_correct a b Ha Hb).
+  intuition.
+  - destruct (cantorCompare a b); auto.
+    + elim (ord_lt_irreflexive x).
+      apply ord_lt_le_trans with y; auto.
+      rewrite Hyb. rewrite <- H. apply Hxa.
+    + elim (ord_lt_irreflexive x).
+      apply ord_lt_le_trans with y; auto.
+      rewrite Hyb. rewrite Hxa. auto with ord.
+  - rewrite H0 in H. rewrite Hxa. rewrite Hyb.
+    auto.
+Qed.
+
+Lemma CNF_le_reflects : reflects CantorNormalForm CNF_denote (Arrow ORD (Arrow ORD PROP)) ord_le CantorNormalForm_le.
+Proof.
+  simpl. intros x [a Ha] Hxa y [b Hb] Hyb.
+  unfold CNF_denote, CantorNormalForm_le in *; simpl in *.
+  generalize (CNF_compare_correct a b Ha Hb).
+  intuition.
+  - rewrite H1 in H.
+    elim (ord_lt_irreflexive x).
+    apply ord_le_lt_trans with y; auto.
+    rewrite Hyb. rewrite Hxa.
+    auto.
+  - destruct (cantorCompare a b); intuition.
+    + rewrite Hxa. rewrite Hyb. auto with ord.
+    + rewrite Hxa. rewrite Hyb. apply H.
+Qed.
+
+
+Definition CF_zero  := CantorSum [].
+Definition CF_one   := CantorSum [ CF_zero ].
+Definition CF_omega := CantorSum [ CF_one ].
+
+Lemma CF_zero_normal : cantorIsNormal CF_zero.
+Proof.
+  simpl. auto.
+Qed.
+
+Lemma CF_one_normal : cantorIsNormal CF_one.
+Proof.
+  simpl. auto.
+Qed.
+
+Lemma CF_omega_normal : cantorIsNormal CF_omega.
+Proof.
+  simpl. auto.
+Qed.
+
+Definition CNF_zero  : CNF := exist _ CF_zero  CF_zero_normal.
+Definition CNF_one   : CNF := exist _ CF_one   CF_one_normal.
+Definition CNF_omega : CNF := exist _ CF_omega CF_omega_normal.
+
+Lemma CNF_reflects_zero : reflects CantorNormalForm CNF_denote ORD 0 CNF_zero.
+Proof.
+  red; simpl.
+  unfold CNF_denote. simpl. reflexivity.
+Qed.
+
+Opaque expOrd.
+Opaque mulOrd.
+Opaque addOrd.
+
+Lemma CNF_reflects_one : reflects CantorNormalForm CNF_denote ORD 1 CNF_one.
+  red; simpl.
+  unfold CNF_denote.
+  simpl.
+  rewrite expOrd_zero.
+  rewrite <- addOrd_zero_r.
+  reflexivity.
+Qed.
+
+Lemma CNF_reflects_omega : reflects CantorNormalForm CNF_denote ORD ω CNF_omega.
+Proof.
+  red; simpl.
+  unfold CNF_denote.
+  simpl.
+  rewrite <- addOrd_zero_r.
+  transitivity (expOrd ω 1).
+  rewrite expOrd_succ.
+  rewrite expOrd_zero.
+  rewrite mulOrd_one_l. reflexivity.
+  apply (index_lt ω 0%nat).
+  split; apply expOrd_monotone.
+  rewrite <- addOrd_zero_r.
+  rewrite expOrd_zero; auto with ord.
+  rewrite <- addOrd_zero_r.
+  rewrite expOrd_zero; auto with ord.
+Qed.
+
+
+Definition cantorIsFinite (x:CF) : option nat :=
+  match x with
+  | CantorSum [] => Some 0%nat
+  | CantorSum (CantorSum [] :: xs) => Some (length xs + 1)%nat
+  | _ => None
+  end.
+
+Lemma cantorIsFinite_fin : forall (x:CF) n,
+    cantorIsNormal x ->
+    cantorIsFinite x = Some n -> x ≈ natOrdSize n.
+Proof.
+  intros [xs] n.
+  destruct xs.
+  - intros H Hn. simpl in Hn. inversion Hn. simpl. reflexivity.
+  - destruct c as [cs]. destruct cs; try discriminate.
+    intros. simpl in H0. inversion H0.
+    simpl.
+    rewrite expOrd_zero.
+    rewrite natOrdSize_add.
+    apply addOrd_eq_mor; try reflexivity.
+    clear n H0 H2.
+    induction xs; simpl; try reflexivity.
+    rewrite IHxs. clear IHxs.
+    assert (Ha : cantorOrd a ≈ 0).
+    { split; auto with ord.
+      simpl in H; intuition.
+      destruct a. destruct l; simpl; auto with ord.
+      intuition. }
+    rewrite Ha.
+    rewrite expOrd_zero.
+    transitivity (natOrdSize (length xs + 1)).
+    { symmetry; apply natOrdSize_add. }
+    replace (length xs + 1)%nat with (1 + length xs)%nat by auto with arith.
+    simpl. reflexivity.
+
+    simpl in H; simpl; destruct xs; intuition.
+    simpl in H4.
+    destruct a; destruct c.
+    destruct l; destruct l0; intuition.
+Qed.
+
+Lemma cantorIsFinite_inf : forall (x:CF),
+    cantorIsFinite x = None -> 1 + x ≈ x.
+Proof.
+  intros [xs].
+  destruct xs; simpl; intuition; try discriminate.
+  destruct c as [cs]; destruct cs; try discriminate.
+  rewrite addOrd_assoc.
+  apply addOrd_eq_mor; try reflexivity.
+  split.
+  - apply additively_closed_collapse.
+    apply expOmega_additively_closed.
+    apply CantorForm_complete.
+    assert (cantorOrd (CantorSum (c::cs)) >= 1).
+    { simpl. rewrite <- addOrd_le1.
+      apply succ_least. apply expOrd_nonzero. }
+    rewrite <- H0.
+    rewrite expOrd_one'.
+    apply (index_lt _ 1%nat).
+    apply (index_lt _ 0%nat).
+  - apply addOrd_le2.
+Qed.
+
+
+Fixpoint cantorSum_add xs ys :=
+  match xs with
+  | [] => ys
+  | (x::xs') =>
+    match cantorSum_add xs' ys with
+    | [] => [x]
+    | (z::zs) => match cantorCompare x z with
+                 | LT => z::zs
+                 | EQ => x::z::zs
+                 | GT => x::z::zs
+                 end
+    end
+  end.
+
+Lemma cantorSum_add_normal xs : forall ys,
+    cantorIsNormal (CantorSum xs) ->
+    cantorIsNormal (CantorSum ys) ->
+    cantorIsNormal (CantorSum (cantorSum_add xs ys)).
+Proof.
+  induction xs; simpl cantorSum_add; intros; auto.
+  assert (cantorIsNormal (CantorSum xs)).
+  { simpl in H; destruct xs; simpl in *; intuition. }
+  generalize (IHxs ys H1 H0).
+  destruct (cantorSum_add xs ys).
+  - simpl in *; intuition.
+  - case_eq (cantorCompare a c); simpl in * ; intuition.
+    rewrite H2 in H3; discriminate.
+    rewrite H2 in H3; discriminate.
+Qed.
+
+Lemma cantorSum_add_correct xs : forall ys,
+    cantorIsNormal (CantorSum xs) ->
+    cantorIsNormal (CantorSum ys) ->
+    cantorOrd (CantorSum xs) + cantorOrd (CantorSum ys) ≈ cantorOrd (CantorSum (cantorSum_add xs ys)).
+Proof.
+  induction xs; simpl cantorSum_add; simpl cantorOrd; intros.
+  - rewrite <- addOrd_zero_l. reflexivity.
+  - assert (cantorIsNormal (CantorSum xs)).
+    { simpl in H; destruct xs; simpl in *; intuition. }
+    generalize (IHxs ys H1 H0).
+    intros. rewrite <- addOrd_assoc.
+    rewrite H2.
+    generalize (cantorSum_add_normal xs ys H1 H0).
+    destruct (cantorSum_add xs ys); simpl cantorOrd.
+    + reflexivity.
+    + case_eq (cantorCompare a c); intros; try reflexivity.
+      simpl fold_right.
+      rewrite addOrd_assoc.
+      apply addOrd_eq_mor; try reflexivity.
+      split.
+      * apply expOrd_add_collapse; auto.
+        apply CantorForm_complete.
+        assert (Ha : cantorIsNormal a).
+        { simpl in H; intuition. }
+        assert (Hc : cantorIsNormal c).
+        { simpl in H4; intuition. }
+        generalize (CNF_compare_correct a c Ha Hc).
+        rewrite H3. auto.
+      * apply addOrd_le2.
+Qed.
+
+Definition CF_add (x y:CF) :=
+  match x, y with
+  | CantorSum xs, CantorSum ys => CantorSum (cantorSum_add xs ys)
+  end.
+
+Lemma CF_add_normal x y :
+  cantorIsNormal x -> cantorIsNormal y -> cantorIsNormal (CF_add x y).
+Proof.
+  destruct x; destruct y; apply cantorSum_add_normal; auto.
+Qed.
+
+Lemma CF_add_correct : forall (x y:CF),
+  cantorIsNormal x ->
+  cantorIsNormal y ->
+  cantorOrd x + cantorOrd y ≈ cantorOrd (CF_add x y).
+Proof.
+  intros [xs] [ys] Hx Hy.
+  apply (cantorSum_add_correct xs ys); auto.
+Qed.
+
+
+Definition CNF_add (x y : CNF) : CNF
+  := exist _ (CF_add (proj1_sig x) (proj1_sig y))
+           (CF_add_normal _ _ (proj2_sig x) (proj2_sig y)).
+
+Lemma CNF_add_reflects : reflects CantorNormalForm CNF_denote (Arrow ORD (Arrow ORD ORD)) addOrd CNF_add.
+Proof.
+  hnf; simpl. unfold CNF_denote. intros x [a Ha] Hxa y [b Hb] Hyb; simpl in *.
+  rewrite Hxa. rewrite Hyb.
+  destruct a as [xs]. destruct b as [ys].
+  apply (cantorSum_add_correct xs ys); auto.
+Qed.
+
+Definition CF_mul_single (x:CF) (e:CF) : CF :=
+  match x, e with
+  | CantorSum [], _  => CantorSum []
+  | _ , CantorSum [] => x
+  | CantorSum (x::_), _ => CantorSum [ CF_add x e ]
+  end.
+
+Definition CF_mul (x:CF) (y:CF) : CF :=
+  match y with
+  | CantorSum ys => fold_right (fun y s => CF_add (CF_mul_single x y) s) CF_zero ys
+  end.
+
+Lemma CF_mul_single_normal : forall x e,
+  cantorIsNormal x ->
+  cantorIsNormal e ->
+  cantorIsNormal (CF_mul_single x e).
+Proof.
+  intros [xs] [es] Hx He.
+  simpl.
+  destruct xs.
+  - simpl; intuition.
+  - destruct es; auto.
+    simpl in *; intuition.
+    apply CF_add_normal; intuition.
+    simpl; auto.
+Qed.
+
+Lemma CF_mul_normal : forall x y,
+  cantorIsNormal x ->
+  cantorIsNormal y ->
+  cantorIsNormal (CF_mul x y).
+Proof.
+  intros x [ys].
+  unfold CF_mul.
+  induction ys.
+  - simpl. auto.
+  - intros.
+    simpl fold_right.
+    apply CF_add_normal.
+    apply (CF_mul_single_normal x a); auto.
+    simpl in H0; intuition.
+    apply IHys; auto.
+    destruct ys; simpl in *; intuition.
+Qed.
+
+Lemma cantorFirstTerm_dominates x xs :
+  cantorIsNormal (CantorSum (x :: xs)) ->
+  cantorOrd (CantorSum xs) ≤ expOrd ω (cantorOrd x) * sz (length xs).
+Proof.
+  induction xs.
+  - simpl; intros; auto with ord.
+  - intros.
+    transitivity (expOrd ω (cantorOrd x) * (natOrdSize (length xs + 1))).
+    + rewrite natOrdSize_add.
+      rewrite ordDistrib_left.
+      rewrite mulOrd_one_r.
+      simpl in *; intuition.
+      apply addOrd_monotone; auto.
+      * apply expOrd_monotone.
+        generalize (CNF_compare_correct x a H0 H).
+        destruct (cantorCompare x a); intuition.
+        apply H2.
+      * apply H4; auto.
+        destruct xs; intuition.
+        assert (cantorOrd a ≤ cantorOrd x).
+        { generalize (CNF_compare_correct x a H0 H).
+          destruct (cantorCompare x a); intuition.
+          apply H7. }
+        assert (cantorOrd c ≤ cantorOrd a).
+        { generalize (CNF_compare_correct a c H H2).
+          destruct (cantorCompare a c); intuition.
+          apply H8. }
+        generalize (CNF_compare_correct x c H0 H2).
+        rewrite H4. intro.
+        apply (ord_lt_irreflexive (cantorOrd x)).
+        apply ord_lt_le_trans with (cantorOrd c); auto.
+        transitivity (cantorOrd a); auto.
+    + apply mulOrd_monotone2.
+      replace (length xs + 1)%nat with (1 + length xs)%nat by auto with arith.
+      simpl; reflexivity.
+Qed.
+
+Lemma CF_mul_single_correct : forall x e,
+  cantorIsNormal x ->
+  cantorIsNormal e ->
+  cantorOrd (CF_mul_single x e) ≈ cantorOrd x * expOrd ω (cantorOrd e).
+Proof.
+  intros [xs] [es] Hx He.
+  destruct xs.
+  - simpl. rewrite mulOrd_zero_l. reflexivity.
+  - destruct es.
+    + simpl fold_right.
+      rewrite expOrd_zero.
+      rewrite mulOrd_one_r.
+      reflexivity.
+    + unfold CF_mul_single.
+      transitivity (expOrd ω (cantorOrd (CF_add c (CantorSum (c0::es))))).
+      { generalize (CF_add c (CantorSum (c0::es))).
+        intros. simpl.
+        rewrite <- addOrd_zero_r. reflexivity. }
+      transitivity (expOrd ω (cantorOrd c + cantorOrd (CantorSum (c0::es)))).
+      { assert (cantorOrd (CF_add c (CantorSum (c0::es))) ≈
+                          (cantorOrd c + cantorOrd (CantorSum (c0 :: es)))).
+        symmetry; apply CF_add_correct; simpl in *; intuition.
+        split; apply expOrd_monotone; apply H. }
+      rewrite expOrd_add.
+      split.
+      * apply mulOrd_monotone1.
+        simpl cantorOrd.
+        apply addOrd_le1.
+      * simpl cantorOrd at 1.
+        apply expOrd_omega_collapse with (length xs).
+        ** apply CantorForm_complete.
+        ** simpl.
+           rewrite <- addOrd_le1.
+           apply expOrd_nonzero.
+        ** apply cantorFirstTerm_dominates; auto.
+Qed.
+
+Lemma CF_mul_correct : forall x y,
+    cantorIsNormal x ->
+    cantorIsNormal y ->
+    cantorOrd (CF_mul x y) ≈ cantorOrd x * cantorOrd y.
+Proof.
+  intros x [ys].
+  induction ys; simpl CF_mul; intros.
+  - simpl cantorOrd.
+    rewrite mulOrd_zero_r. reflexivity.
+  - simpl cantorOrd.
+    rewrite ordDistrib_left.
+    rewrite <- CF_add_correct.
+    apply addOrd_eq_mor.
+    apply CF_mul_single_correct; auto.
+    simpl in H0; intuition.
+    apply IHys; auto.
+    destruct ys; simpl in * ; intuition.
+    apply CF_mul_single_normal; auto.
+    simpl in H0; intuition.
+    apply (CF_mul_normal x (CantorSum ys)); auto.
+    destruct ys; simpl in * ; intuition.
+Qed.
+
+Definition CNF_mul (x y : CNF) : CNF
+  := exist _ (CF_mul (proj1_sig x) (proj1_sig y))
+           (CF_mul_normal _ _ (proj2_sig x) (proj2_sig y)).
+
+Lemma CNF_mul_reflects : reflects CantorNormalForm CNF_denote (Arrow ORD (Arrow ORD ORD)) mulOrd CNF_mul.
+Proof.
+  hnf; simpl. unfold CNF_denote. intros x [a Ha] Hxa y [b Hb] Hyb; simpl in *.
+  rewrite Hxa. rewrite Hyb.
+  symmetry. apply CF_mul_correct; auto.
+Qed.
+
+
+Definition CF_nat (n:nat) : CF := CantorSum (repeat CF_zero n).
+
+Lemma CF_nat_normal : forall n, cantorIsNormal (CF_nat n).
+Proof.
+  induction n; simpl; intuition.
+  destruct n; simpl in *; intuition.
+  discriminate.
+Qed.
+
+Lemma CF_nat_correct : forall n, CF_nat n ≈ natOrdSize n.
+Proof.
+  induction n; simpl; try reflexivity.
+  rewrite expOrd_zero.
+  rewrite IHn.
+  transitivity (natOrdSize (n+1)%nat).
+  rewrite natOrdSize_add. reflexivity.
+  replace (n+1)%nat with (1+n)%nat by auto with arith.
+  simpl. reflexivity.
+Qed.
+
+
+Definition CF_exp_single (x:CF) (e:CF) : CF :=
+  match x with
+
+    (* 0 ^ (ω^e) = 1 *)
+  | CantorSum [] => CF_one
+
+    (* 1 ^ (ω^e) = 1 *)
+  | CantorSum [ CantorSum [] ] => CF_one
+
+  | CantorSum (CantorSum [] :: _ ) =>
+    match cantorIsFinite e with
+      (* n ^ (ω^0) = n *)
+    | Some 0 => x
+
+      (* n ^ (ω^(1+m)) = ω^(ω^m) for finite n > 1, finite m *)
+    | Some (S m) => CantorSum [CantorSum [ CF_nat m ]]
+
+      (* n ^ (ω^e) = ω^(ω^e)  for e >= ω, finite n > 1 *)
+    | None => CantorSum [CantorSum [e]]
+    end
+
+  | CantorSum (x1 :: _) =>
+    match cantorIsFinite e with
+      (* x^ (ω^0) = x *)
+    | Some 0 => x
+
+      (* (ω^x₁ + b) ^ (ω^e) = ω^(x₁ * ω^e)  when x₁ >= 1, e > 0 *)
+    | _ => CantorSum [ CF_mul x1 (CantorSum [e]) ]
+    end
+  end.
+
+Definition CF_exp (x:CF) (y:CF) : CF :=
+  match y with
+  | CantorSum ys => fold_right (fun y s => CF_mul (CF_exp_single x y) s) CF_one ys
+  end.
+
+Opaque CF_add.
+Opaque CF_mul.
+
+Lemma CF_exp_single_normal e x :
+  cantorIsNormal x ->
+  cantorIsNormal e ->
+  cantorIsNormal (CF_exp_single x e).
+Proof.
+  intros. unfold CF_exp_single.
+  destruct x as [xs].
+  destruct xs as [|x xs].
+  { apply CF_one_normal. }
+  destruct x as [ls].
+  destruct ls as [|l ls].
+  - destruct xs.
+    + apply CF_one_normal.
+    + destruct (cantorIsFinite e).
+      destruct n; auto.
+      * generalize (CF_nat_normal n).
+        simpl; intuition.
+      * simpl; intuition.
+  - destruct (cantorIsFinite e).
+    destruct n; auto.
+    simpl; intuition.
+    apply CF_mul_normal; simpl in *; intuition.
+    simpl; intuition.
+    apply CF_mul_normal; simpl in *; intuition.
+Qed.
+
+Lemma CF_exp_normal x y :
+  cantorIsNormal x ->
+  cantorIsNormal y ->
+  cantorIsNormal (CF_exp x y).
+Proof.
+  destruct y as [ys]. induction ys; simpl; intuition.
+  apply CF_mul_normal; auto.
+  apply CF_exp_single_normal; auto.
+  apply H0. destruct ys; simpl in *; intuition.
+Qed.
+
+Lemma CF_exp_single_correct x e :
+  cantorIsNormal x ->
+  cantorIsNormal e ->
+  cantorOrd (CF_exp_single x e) ≈ expOrd (cantorOrd x) (expOrd ω (cantorOrd e)).
+Proof.
+  unfold CF_exp_single. intros.
+  destruct x as [xs].
+  destruct e as [es].
+  destruct xs as [|x xs].
+  - simpl; intros.
+    rewrite <- addOrd_zero_r.
+    rewrite expOrd_zero.
+    split.
+    apply succ_least. apply expOrd_nonzero.
+    rewrite expOrd_unfold.
+    apply lub_least; auto with ord.
+    apply sup_least. intro i.
+    rewrite mulOrd_zero_r.
+    apply ord_lt_le; apply succ_lt.
+  - destruct x as [ls].
+    destruct ls as [|l ls].
+    destruct xs.
+    + simpl.
+      rewrite <- addOrd_zero_r.
+      rewrite expOrd_zero.
+      symmetry; apply expOrd_one_base.
+    + case_eq (cantorIsFinite (CantorSum es)). intros n Hn.
+      * rewrite (cantorIsFinite_fin (CantorSum es) n H0 Hn).
+        destruct n.
+        ** rewrite expOrd_zero.
+           rewrite expOrd_one'. reflexivity.
+           simpl. rewrite <- addOrd_le1.
+           apply expOrd_nonzero.
+        ** rewrite (cantorIsFinite_fin (CantorSum (CantorSum [] :: c :: xs)) _ H (refl_equal _)).
+           change (S n) with (1+n)%nat.
+           replace (1+n)%nat with (n+1)%nat by auto with arith.
+           rewrite (natOrdSize_add n).
+           rewrite expNatToOmegaPow.
+           rewrite <- CF_nat_correct.
+           simpl.
+           repeat rewrite <- addOrd_zero_r.
+           reflexivity.
+           simpl.
+           rewrite ord_lt_unfold; exists tt. simpl.
+           rewrite natOrdSize_add.
+           apply addOrd_le1.
+      * intros.
+        rewrite (cantorIsFinite_fin (CantorSum (CantorSum [] :: c :: xs)) _ H (refl_equal _)).
+        symmetry.
+        simpl cantorOrd.
+        repeat rewrite <- addOrd_zero_r.
+        apply expNatToOmegaInf.
+        ** simpl.
+           rewrite ord_lt_unfold; exists tt. simpl.
+           rewrite natOrdSize_add.
+           apply addOrd_le1.
+        ** rewrite (cantorIsFinite_inf (CantorSum es) H1).
+           reflexivity.
+    + cut (cantorOrd (CantorSum es) > 0 ->
+           cantorOrd (CantorSum [CF_mul (CantorSum (l :: ls)) (CantorSum [CantorSum es])]) ≈
+                     expOrd (cantorOrd (CantorSum (CantorSum (l :: ls) :: xs)))
+                     (expOrd ω (cantorOrd (CantorSum es)))).
+      { intros Hmain.
+        case_eq (cantorIsFinite (CantorSum es)).
+        - intros n Hn.
+          destruct n.
+          + rewrite (cantorIsFinite_fin (CantorSum es) 0%nat H0 Hn).
+            rewrite expOrd_zero.
+            rewrite expOrd_one'.
+            reflexivity.
+            simpl.
+            rewrite <- addOrd_le1.
+            apply expOrd_nonzero.
+          + apply Hmain.
+            rewrite (cantorIsFinite_fin (CantorSum es) (S n) H0 Hn).
+            simpl.
+            rewrite ord_lt_unfold; exists tt; auto with ord.
+        - intro. apply Hmain.
+          rewrite <- (cantorIsFinite_inf (CantorSum es) H1).
+          rewrite <- addOrd_le1.
+          apply succ_lt. }
+      intro.
+      simpl cantorOrd at 1.
+      rewrite CF_mul_correct.
+      rewrite <- addOrd_zero_r.
+      rewrite expOrd_mul.
+      split.
+      * simpl. rewrite <- addOrd_zero_r.
+        apply expOrd_monotone_base.
+        apply addOrd_le1.
+      * simpl.
+        repeat rewrite <- addOrd_zero_r.
+        apply expToOmega_collapse_tower with (length xs); auto.
+        ** transitivity (expOrd ω 1).
+           { rewrite expOrd_one'.
+             transitivity (natOrdSize (1+length xs)).
+             rewrite natOrdSize_add. reflexivity.
+             apply index_le.
+             apply (index_lt _ 0%nat). }
+           apply expOrd_monotone.
+           rewrite <- addOrd_le1.
+           apply succ_least. apply expOrd_nonzero.
+        ** change (cantorOrd (CantorSum xs) ≤
+                       expOrd ω (cantorOrd (CantorSum (l::ls))) * sz (length xs)).
+           apply cantorFirstTerm_dominates; auto.
+        ** apply (CantorForm_complete (CantorSum es)).
+      * simpl in *; intuition.
+      * simpl; intuition.
+Qed.
+
+Lemma CF_exp_correct : forall x y,
+  cantorIsNormal x ->
+  cantorIsNormal y ->
+  cantorOrd (CF_exp x y) ≈ expOrd (cantorOrd x) (cantorOrd y).
+Proof.
+  intros x [ys]. induction ys; simpl; intuition.
+  - do 2 rewrite expOrd_zero. rewrite <- addOrd_zero_r. reflexivity.
+  - rewrite CF_mul_correct.
+    + rewrite CF_exp_single_correct; auto.
+      rewrite expOrd_add.
+      apply mulOrd_eq_mor; try reflexivity.
+      apply H0.
+      destruct ys; intuition.
+      simpl; intuition.
+    + apply CF_exp_single_normal; auto.
+    + apply (CF_exp_normal x (CantorSum ys)); auto.
+      destruct ys; intuition.
+      simpl; intuition.
+Qed.
+
+Definition CNF_exp (x y:CNF) : CNF :=
+  exist _ (CF_exp (proj1_sig x) (proj1_sig y))
+          (CF_exp_normal _ _ (proj2_sig x) (proj2_sig y)).
+
+Theorem CNF_exp_reflects : reflects CantorNormalForm CNF_denote (Arrow ORD (Arrow ORD ORD)) expOrd CNF_exp.
+Proof.
+  hnf; simpl. unfold CNF_denote. intros x [a Ha] Hxa y [b Hb] Hyb; simpl in *.
+  rewrite Hxa. rewrite Hyb.
+  symmetry. apply CF_exp_correct; auto.
+Qed.
+
+
+Theorem CNF_reflects_KnuthUp2_impossible :
+  ~exists f, reflects CantorNormalForm CNF_denote (Arrow ORD (Arrow ORD ORD)) (KnuthUp 2) f.
+Proof.
+  intros [f Hf].
+  hnf in Hf.
+  specialize (Hf ω CNF_omega CNF_reflects_omega).
+  hnf in Hf.
+  specialize (Hf ω CNF_omega CNF_reflects_omega).
+  red in Hf.
+  rewrite KnuthUp_epsilon in Hf.
+  apply (ord_lt_irreflexive (ε 0)).
+  rewrite Hf at 1.
+  apply cantorForm_below_epsilon.
+Qed.
+
+
+Lemma CNF_limit : limitOrdinal CNF.
+Proof.
+  red. simpl. split.
+  exact (inhabits CNF_zero).
+  hnf. simpl; intros.
+  exists (CNF_add a CNF_one).
+  destruct a as [a Ha]; simpl.
+  unfold CNF_denote; simpl.
+  rewrite <- CF_add_correct; auto.
+  simpl.
+  rewrite <- addOrd_zero_r.
+  rewrite expOrd_zero.
+  Transparent addOrd. unfold addOrd. Opaque addOrd.
+  rewrite foldOrd_succ. rewrite foldOrd_zero.
+  apply succ_lt.
+  intros. rewrite H. apply ord_lt_le; apply succ_lt.
+  apply CF_one_normal.
+Qed.
+
+Theorem CNF_expOmega_fixpoint : expOrd ω CNF ≤ CNF.
+Proof.
+  transitivity (expOrd ω (supOrd CNF_denote)).
+  - apply expOrd_monotone.
+    apply ord_isLimit.
+    apply CNF_limit.
+  - etransitivity; [ apply expOrd_continuous |].
+    exact CNF_zero.
+    apply sup_least; intro cnf.
+    transitivity (CNF_denote (CNF_exp CNF_omega cnf)).
+    unfold CNF_denote.
+    simpl.
+    rewrite CF_exp_correct.
+    apply expOrd_monotone_base.
+    apply CNF_reflects_omega.
+    apply CF_omega_normal.
+    apply proj2_sig.
+    apply index_le.
+Qed.
+
+Theorem CNF_is_ε0 : CNF ≈ ε 0.
+Proof.
+  split.
+  - rewrite ord_le_unfold; intro cnf.
+    apply cantorForm_below_epsilon.
+  - apply ε0_least_expOmega_closed.
+    apply CNF_expOmega_fixpoint.
+Qed.
+
+Remark ε0_least_exp_closed :
+  forall X denote zeroX succX expOmegaX,
+    reflects X denote ORD 0 zeroX ->
+    reflects X denote (Arrow ORD ORD) succOrd succX ->
+    reflects X denote (Arrow ORD ORD) (expOrd ω) expOmegaX ->
+
+    ε 0 ≤ ord X denote.
+Proof.
+  intros X denote zeroX succX expOmegaX Hzero Hsucc HexpOmega.
+
+  assert (Hlimit : limitOrdinal (ord X denote)).
+  { simpl; split.
+    - exact (inhabits zeroX).
+    - hnf; simpl; intros.
+      exists (succX a).
+      apply ord_lt_le_trans with (succOrd (denote a)).
+      apply succ_lt.
+      apply Hsucc.
+      simpl; reflexivity. }
+  
+  apply ε0_least_expOmega_closed; auto.
+  transitivity (expOrd ω (supOrd denote)).
+  - apply expOrd_monotone.
+    apply ord_isLimit; auto.
+  - etransitivity; [ apply expOrd_continuous |].
+    exact zeroX.
+    apply sup_least; intro x.
+    transitivity (denote (expOmegaX x)).
+    apply HexpOmega. simpl; reflexivity.
+    apply (index_le (ord X denote)).
+Qed.
+
+
+Require Import ClassicalFacts.
+From Ordinal Require Import Classical.
+
+Theorem CNF_has_enough_notations (EM:excluded_middle) :
+  forall x, x < ε 0 -> exists c:CNF, x ≈ c.
+Proof.
+  intros.
+  induction x using ordinal_induction.
+  destruct (cantor_decomposition EM x) as [ls [H1 H2]].
+  cut (exists ca:CNF, cantor_denote ls ≈ sz ca).
+  { intros. destruct H3 as [ca Hca] ; auto.
+    exists ca. rewrite <- H2. auto. }
+
+  destruct H2. clear H3.
+  induction ls; intros.
+  - simpl.
+    exists CNF_zero.
+    reflexivity.
+  - simpl.
+    assert (a < x).
+    { destruct (classical.order_total EM x a); auto.
+      elim (ord_lt_irreflexive (ε 0)).
+      apply ord_le_lt_trans with x; auto.
+      simpl. unfold fixOrd.
+      apply sup_least. intro i.
+      induction i; simpl.
+      - rewrite ord_le_unfold; intros [].
+      - unfold powOmega.
+        rewrite IHi.
+        simpl in H1. destruct H1.
+        rewrite <- H2 at 2.
+        simpl.
+        rewrite <- addOrd_le1.
+        apply expOrd_monotone; auto. }
+
+    destruct (H0 a H3) as [ac Hac].
+    transitivity x; auto.
+    destruct IHls as [cls Hcls]; auto.
+    simpl in H1; intuition.
+    destruct ls; simpl in *; intuition.
+    transitivity a; auto.
+    simpl in H2.
+    rewrite <- H2.
+    apply addOrd_le2.
+    exists (CNF_add (CNF_exp CNF_omega ac) cls).
+    apply CNF_add_reflects; auto.
+    apply CNF_exp_reflects; auto.
+    apply CNF_reflects_omega.
+Qed.
+
+Theorem CNF_has_enough_notations_is_classical :
+  (forall x, x < ε 0 -> exists c:CNF, x ≈ c) ->
+  excluded_middle.
+Proof.
+  intros H P.
+  destruct (H (classical.truth_ord P)).
+  - simpl. unfold fixOrd.
+    rewrite <- (sup_le _ _ 2%nat).
+    unfold iter_f.
+    unfold powOmega.
+    apply ord_lt_le_trans with ω.
+    rewrite ord_lt_unfold.
+    exists 1%nat.
+    simpl.
+    unfold classical.truth_ord.
+    rewrite ord_le_unfold.
+    simpl; intros.
+    apply succ_lt.
+    transitivity (expOrd ω 1).
+    rewrite expOrd_one'. reflexivity.
+    apply (index_lt _ 0%nat).
+    apply expOrd_monotone.
+    apply succ_least. apply expOrd_nonzero.
+
+  - destruct x as [x Hx].
+    simpl in *. unfold CNF_denote in H0.
+    simpl in *.
+    destruct x as [xs].
+    destruct xs as [|x xs]; simpl in *.
+    + right; intro HP.
+      destruct H0.
+      rewrite ord_le_unfold in H0.
+      specialize (H0 HP).
+      rewrite ord_lt_unfold in H0.
+      destruct H0 as [[] _].
+    + left.
+      assert (0 < classical.truth_ord P).
+      { rewrite H0.
+        rewrite <- addOrd_le1.
+        apply expOrd_nonzero. }
+      rewrite ord_lt_unfold in H1.
+      destruct H1 as [HP _]; auto.
+Qed.
+
+Theorem CNF_has_enough_notations_is_classical_for_complete_ordinals :
+  (forall x, complete x -> x < ε 0 -> exists c:CNF, x ≈ c) ->
+  excluded_middle.
+Proof.
+  intros H P.
+  destruct (H (classical.truth_ord' P)).
+  - apply classical.truth_ord'_complete.
+  - simpl.
+    unfold fixOrd.
+    rewrite <- (sup_le _ _ 3%nat).
+    unfold iter_f.
+    unfold powOmega.
+    apply ord_le_lt_trans with ω.
+    unfold classical.truth_ord'.
+    apply sup_least.
+    intro n.
+    apply lub_least.
+    apply (index_le _ 1%nat).
+    rewrite ord_le_unfold; intro  HP.
+    simpl.
+    apply index_lt.
+    apply ord_le_lt_trans with (expOrd ω 1).
+    rewrite expOrd_one'. auto with ord.
+    apply (index_lt _ 0%nat).
+    apply expOrd_increasing.
+    apply (index_lt _ 1%nat).
+    apply ord_lt_le_trans with (expOrd ω 1).
+    rewrite expOrd_one'.
+    apply (index_lt _ 1%nat).
+    apply (index_lt _ 0%nat).
+    apply expOrd_monotone.
+    apply succ_least. apply expOrd_nonzero.
+  - case_eq (cantorIsFinite (proj1_sig x)).
+    + intros.
+      right; intro.
+      simpl in H0.
+      unfold CNF_denote in  H0.
+      apply cantorIsFinite_fin in H1.
+      rewrite H1 in H0.
+      destruct H0.
+      apply (ord_lt_irreflexive ω).
+      apply ord_le_lt_trans with (natOrdSize n).
+      rewrite <- H0.
+      unfold classical.truth_ord'.
+      rewrite ord_le_unfold; intro i.
+      rewrite <- (sup_le _ _ i).
+      rewrite <- lub_le2.
+      rewrite ord_lt_unfold. exists H2.
+      simpl. reflexivity.
+      apply index_lt.
+      apply proj2_sig.
+    + intro. left.
+      destruct H0.
+      assert (1 < classical.truth_ord' P).
+      apply cantorIsFinite_inf in H1.
+      apply ord_lt_le_trans with (sz x); auto.
+      simpl.
+      unfold CNF_denote.
+      rewrite <- H1.
+      rewrite <- H1.
+      rewrite addOrd_assoc.
+      rewrite <- addOrd_le1.
+      Transparent addOrd. unfold addOrd. Opaque addOrd.
+      rewrite foldOrd_succ.
+      rewrite foldOrd_zero.
+      apply succ_lt.
+      intros. rewrite H3. apply ord_lt_le. apply succ_lt.
+      rewrite ord_lt_unfold in H3.
+      destruct H3 as [[n q] Hq]; simpl in *.
+      destruct q.
+      elim (ord_lt_irreflexive 1); auto with ord.
+      apply ord_le_lt_trans with 0; auto.
+      apply succ_lt.
+      auto.
+Qed.
