Ordinal/Reflection.v
@@ -1,0 +1,43 @@
+Require Import Morphisms.
+Require Import Coq.Program.Basics.
+Require Import NArith.
+Require Import List.
+
+Unset Printing Records.
+
+From Ordinal Require Import Defs.
+From Ordinal Require Import Operators.
+From Ordinal Require Import Arith.
+From Ordinal Require Import Cantor.
+From Ordinal Require Import Fixpoints.
+
+Open Scope ord_scope.
+
+Inductive Shape : Set :=
+| PROP : Shape
+| ORD : Shape
+| Arrow : Shape -> Shape -> Shape
+.
+
+Fixpoint ordShape (S:Shape) : Type :=
+  match S with
+  | PROP        => Prop
+  | ORD         => Ord
+  | Arrow S1 S2 => ordShape S1 -> ordShape S2
+  end.
+
+Fixpoint reflShape (S:Shape) (X:Type) : Type :=
+  match S with
+  | PROP        => Prop
+  | ORD         => X
+  | Arrow S1 S2 => reflShape S1 X -> reflShape S2 X
+  end.
+
+Fixpoint reflects (A:Type) (f:A -> Ord) (S:Shape) : ordShape S -> reflShape S A -> Prop :=
+  match S as S' return ordShape S' -> reflShape S' A -> Prop with
+  | PROP => fun p q => p <-> q
+  | ORD  => fun x a => x ≈ f a
+  | Arrow S1 S2 => fun g h => forall x a, reflects A f S1 x a -> reflects A f S2 (g x) (h a)
+  end.
+
+
